

Pfaffian Differential Equations Assignment - Page 33

Tek Raj Pant

July 16, 2025

1 Part 2 - Page 33

Verify that the following equations are integrable and find their primitives

1.1 $2y(a-x)dx + [z - y^2 + (a-x)^2]dy - ydz = 0$

We are given the PfDE

$$2y(a-x)dx + [z - y^2 + (a-x)^2]dy - ydz = 0 \quad (1)$$

Let's define the vector $\vec{X} = (P, Q, R)$, where $P = 2y(a-x)$, $Q = z - y^2 + (a-x)^2$, $R = -y$ so $\vec{X} = (2y(a-x), z - y^2 + (a-x)^2, -y)$.

To check the integrability, let's calculate the $\vec{X} \cdot (\nabla \times \vec{X})$

$$\vec{X} \cdot (\nabla \times \vec{X}) = \begin{vmatrix} P & Q & R \\ \frac{\partial}{\partial x} & \frac{\partial}{\partial y} & \frac{\partial}{\partial z} \\ P & Q & R \end{vmatrix}$$

$$\vec{X} \cdot (\nabla \times \vec{X}) = \begin{vmatrix} 2y(a-x) & (z - y^2 + (a-x)^2) & -y \\ \frac{\partial}{\partial x} & \frac{\partial}{\partial y} & \frac{\partial}{\partial z} \\ 2y(a-x) & (z - y^2 + (a-x)^2) & -y \end{vmatrix}$$

$$\vec{X} \cdot (\nabla \times \vec{X}) = 2y(a-x)(-1-1) + (z - y^2 + (a-x)^2)(0-0) - y(-2(a-x) - 2a + 2x)$$

$$\vec{X} \cdot (\nabla \times \vec{X}) = -4y(a-x) - y(-2a + 2x - 2a + 2x)$$

$$\vec{X} \cdot (\nabla \times \vec{X}) = -4y(a-x) - y(-4a + 4x)$$

$$\vec{X} \cdot (\nabla \times \vec{X}) = -4ay + 4xy + 4ay - 4xy$$

$$\vec{X} \cdot (\nabla \times \vec{X}) = 0$$

(2)

Since $\vec{X} \cdot \text{curl } \vec{X} = 0$, the given Pfaffian Differential Equation (1) is integrable. Dividing the given PfDE by y^2 on both sides

$$\begin{aligned} \frac{2}{y}(a-x)dx + \frac{z}{y^2}dy - dy + \frac{(a-x)^2}{y^2}dy - \frac{1}{y}dz &= 0 \\ \frac{2}{y}(a-x)dx + \frac{(a-x)^2}{y^2}dy + \frac{z}{y^2}dy - dy - \frac{1}{y}dz &= 0 \end{aligned} \quad (3)$$

Here the terms $\frac{2}{y}(a-x)dx + \frac{(a-x)^2}{y^2}dy$ can be written as the differential of $-\frac{(a-x)^2}{y}$

$$d\left(-\frac{(a-x)^2}{y}\right) = -d\left(\frac{(a-x)^2}{y}\right) = \frac{2}{y}(a-x)dx + \frac{(a-x)^2}{y^2}dy$$

Also the remaining terms $\frac{z}{y^2}dy - \frac{1}{y}dz - dy$ can be written as the differential of $(-\frac{z}{y} - y)$

$$d\left(-\frac{z}{y} - y\right) = -\left(\frac{z}{y^2}dy + \frac{1}{y}dz\right) - dy = \frac{z}{y^2}dy - \frac{1}{y}dz - dy$$

Thus the equation (3) becomes

$$d\left(-\frac{(a-x)^2}{y}\right) + d\left(-\frac{z}{y} - y\right) = 0$$

Combining the differentials:

$$\begin{aligned} d\left(-\frac{(a-x)^2}{y} - \frac{z}{y} - y\right) &= 0 \\ d\left(\frac{(a-x)^2}{y} + \frac{z}{y} + y\right) &= 0 \end{aligned}$$

Integrating on both sides

$$\frac{(a-x)^2}{y} + \frac{z}{y} + y = C, \text{ where } C \text{ is an arbitrary constant.}$$

This is the required primitives of the given PfDE.

$$\mathbf{1.2} \quad y(1+z^2)dx - x(1+z^2)dy + (x^2+y^2)dz = 0$$

We are given the PfDE

$$y(1+z^2)dx - x(1+z^2)dy + (x^2+y^2)dz = 0 \quad (1)$$

Let's define the vector $\vec{X} = (P, Q, R)$, where $P = y(1+z^2)$, $Q = -x(1+z^2)$, $R = x^2+y^2$ so $\vec{X} = (y(1+z^2), -x(1+z^2), x^2+y^2)$.

To check the integrability, let's calculate the $\vec{X} \cdot (\nabla \times \vec{X})$

$$\begin{aligned} \vec{X} \cdot (\nabla \times \vec{X}) &= \begin{vmatrix} P & Q & R \\ \frac{\partial}{\partial x} & \frac{\partial}{\partial y} & \frac{\partial}{\partial z} \\ P & Q & R \end{vmatrix} \\ \vec{X} \cdot (\nabla \times \vec{X}) &= \begin{vmatrix} y(1+z^2) & -x(1+z^2) & x^2+y^2 \\ \frac{\partial}{\partial x} & \frac{\partial}{\partial y} & \frac{\partial}{\partial z} \\ y(1+z^2) & -x(1+z^2) & x^2+y^2 \end{vmatrix} \\ \vec{X} \cdot (\nabla \times \vec{X}) &= y(1+z^2)(2y+2xz) + x(1+z^2)(2x-2yz) + (x^2+y^2)(-1-z^2-1-z^2) \\ \vec{X} \cdot (\nabla \times \vec{X}) &= (1+z^2)(2y^2-2xyz+2x^2+2xyz) - 2(x^2+y^2)(1+z^2) \\ \vec{X} \cdot (\nabla \times \vec{X}) &= (1+z^2)(2y^2+2x^2-2x^2-2y^2) \\ \vec{X} \cdot (\nabla \times \vec{X}) &= 0 \end{aligned}$$

Since $\vec{X} \cdot \text{curl } \vec{X} = 0$, the given Pfaffian Differential Equation (1) is integrable.

Dividing the given PfDE by $(x^2+y^2)(1+z^2)$, we get

$$\frac{y}{x^2+y^2}dx - \frac{x}{x^2+y^2}dy + \frac{1}{1+z^2}dz = 0$$

The terms $\frac{y}{x^2+y^2} - \frac{x}{x^2+y^2}$ can be expressed as the differential $d(-\tan^{-1} \frac{y}{x})$

$$-d(\tan^{-1} \frac{y}{x}) = -(\frac{xdy - ydx}{x^2+y^2})$$

Also $d(\tan^{-1} z) = \frac{dz}{1+z^2}$

Hence the equation becomes

$$-d(\tan^{-1} \frac{y}{x}) + d(\tan^{-1} z) = 0$$

Integrating both sides we get

$$\tan^{-1} z - \tan^{-1} \frac{y}{x} = C, \text{ where } C \text{ is an arbitrary constant}$$

This is the require primitives

$$\mathbf{1.3} \quad (y^2 + yz + z^2)dx + (z^2 + zx + x^2)dy + (x^2 + xy + y^2)dz = 0$$

We are given the PfDE

$$(y^2 + yz + z^2)dx + (z^2 + zx + x^2)dy + (x^2 + xy + y^2)dz = 0 \quad (1)$$

Let's define the vector $\vec{X} = (P, Q, R)$, where $P = (y^2 + yz + z^2)$

$Q = (z^2 + zx + x^2)$, $R = (x^2 + xy + y^2)$

So $\vec{X} = ((y^2 + yz + z^2), (z^2 + zx + x^2), (x^2 + xy + y^2))$.

To check the integrability, lets calculate the $\vec{X} \cdot (\nabla \times \vec{X})$

$$\begin{aligned} \vec{X} \cdot (\nabla \times \vec{X}) &= \begin{vmatrix} P & Q & R \\ \frac{\partial}{\partial x} & \frac{\partial}{\partial y} & \frac{\partial}{\partial z} \\ P & Q & R \end{vmatrix} \\ \vec{X} \cdot (\nabla \times \vec{X}) &= \begin{vmatrix} (y^2 + yz + z^2) & (z^2 + zx + x^2) & (x^2 + xy + y^2) \\ \frac{\partial}{\partial x} & \frac{\partial}{\partial y} & \frac{\partial}{\partial z} \\ (y^2 + yz + z^2) & (z^2 + zx + x^2) & (x^2 + xy + y^2) \end{vmatrix} \\ \vec{X} \cdot (\nabla \times \vec{X}) &= (y^2 + yz + z^2)(2y - 2z) + (z^2 + zx + x^2)(2z - 2x) \\ &\quad + (x^2 + xy + y^2)(2x - 2y) \\ \vec{X} \cdot (\nabla \times \vec{X}) &= 2y^3 + 2y^2z + 2yz^2 - 2y^2z - 2yz^2 - 2z^3 \\ &\quad + 2z^3 + 2z^2x + 2zx^2 - 2zx^2 - 2x^3 - 2zx^2 \\ &\quad + 2x^3 + 2x^2y + 2xy^2 - 2x^2y - 2xy^2 - 2y^3 \\ \vec{X} \cdot (\nabla \times \vec{X}) &= 0 \end{aligned}$$

Since $\vec{X} \cdot \text{curl } \vec{X} = 0$, the given Pfaffian Differential Equation (1) is integrable.

Since the given PfDE is homogeneous of degree 2

Let $y = ux$ and $z = vx$

$$dy = udx + xdu$$

$$dz = vdx + xdv$$

Then the given PfDE becomes

$$\begin{aligned}
& x^2(u^2 + uv + v^2) dx + x^2u(v^2 + v + 1) dx + x^2v(u^2 + u + 1) dx \\
& + x^3(v^2 + v + 1) du + x^3(u^2 + u + 1) dv = 0 \\
& x^2 \left[(u^2 + uv + v^2) + u(v^2 + v + 1) + v(u^2 + u + 1) \right] dx \\
& + x^3(v^2 + v + 1) du + x^3(u^2 + u + 1) dv = 0. \\
& x^2 \left[(u + v + 1)(u + uv + v) \right] dx \\
& + x^3(v^2 + v + 1) du \\
& + x^3(u^2 + u + 1) dv = 0.
\end{aligned}$$

Dividing both sides by $\frac{1}{x^3 \left[(u+v+1)(u+uv+v) \right]}$

$$\frac{1}{x} dx + \frac{v^2 + v + 1}{(u + v + 1)(u + uv + v)} du + \frac{u^2 + u + 1}{(u + v + 1)(u + uv + v)} dv = 0$$

Using Partial Fraction

$$\begin{aligned}
\frac{v^2 + v + 1}{(u + v + 1)(u + uv + v)} &= \frac{v + 1}{u + uv + v} - \frac{1}{u + v + 1} \\
\frac{u^2 + u + 1}{(u + v + 1)(u + uv + v)} &= \frac{u + 1}{u + uv + v} - \frac{1}{u + v + 1}
\end{aligned}$$

So,

$$\frac{1}{x} dx + \frac{v + 1}{u + uv + v} du - \frac{1}{u + uv + v} du + \frac{u + 1}{u + uv + v} dv - \frac{1}{u + v + 1} dv = 0$$

Integrating we get

$\ln(x) + \ln(u + uv + v) - \ln(u + v + 1) + \ln(u + uv + v) - \ln(u + v + 1) = C$,
where C is an arbitrary constant

$$\ln \left(x \left(\frac{u + uv + v}{u + v + 1} \right)^2 \right) = C$$

Exponentiating both sides:

$$x \left(\frac{u + uv + v}{u + v + 1} \right)^2 = e^C = C_1$$

Substituting $u = \frac{y}{x}$, $v = \frac{z}{x}$:

$$\begin{aligned} x \left(\frac{\frac{y}{x} + \frac{y}{x} \cdot \frac{z}{x} + \frac{z}{x}}{\frac{y}{x} + \frac{z}{x} + 1} \right)^2 &= C_1 \\ &= x \left(\frac{\frac{y+z}{x} + \frac{yz}{x^2}}{\frac{y+z+x}{x}} \right)^2 \\ &= x \left(\frac{y+z + \frac{yz}{x}}{y+z+x} \cdot \frac{1}{x} \right)^2 \\ &= x \left(\frac{yx + zx + yz}{x(y+z+x)} \right)^2 \\ &= x \cdot \left(\frac{yx + yz + zx}{x(y+z+x)} \right)^2 \\ &= \frac{(yx + yz + zx)^2}{x(y+z+x)^2} = C_1 \\ &\Rightarrow \left(\frac{yx + yz + zx}{y+z+x} \right)^2 = C_1 x \end{aligned}$$

Hence, the required primitive is:

$$\boxed{\left(\frac{yx + yz + zx}{y+z+x} \right)^2 = C_1 x}$$

1.4 $yz dx + xz dy + xy dz = 0$

We are given the Pfaffian differential equation:

$$yz dx + xz dy + xy dz = 0 \tag{1}$$

Define the vector $\vec{X} = (P, Q, R)$, where:

$$P = yz, \quad Q = xz, \quad R = xy$$

Let's compute $\vec{X} \cdot (\nabla \times \vec{X})$:

$$\vec{X} \cdot (\nabla \times \vec{X}) = \begin{vmatrix} P & Q & R \\ \frac{\partial}{\partial x} & \frac{\partial}{\partial y} & \frac{\partial}{\partial z} \\ P & Q & R \end{vmatrix}$$

Expanding the determinant:

$$\vec{X} \cdot (\nabla \times \vec{X}) = yz \left(\frac{\partial}{\partial y}(xy) - \frac{\partial}{\partial z}(xz) \right) - xz \left(\frac{\partial}{\partial x}(xy) - \frac{\partial}{\partial z}(yz) \right) + xy \left(\frac{\partial}{\partial x}(xz) - \frac{\partial}{\partial y}(yz) \right)$$

$$\vec{X} \cdot (\nabla \times \vec{X}) = yz(x - x) - xz(y - y) + xy(z - z) = 0$$

Since $\vec{X} \cdot (\nabla \times \vec{X}) = 0$, the given Pfaffian differential equation is **integrable**.

The left-hand side expression can be written as:

$$yz \, dx + xz \, dy + xy \, dz = d(xyz)$$

Hence, the equation becomes:

$$d(xyz) = 0$$

Integrating both sides:

$$xyz = C, \quad \text{where } C \text{ is an arbitrary constant.}$$

This is the general solution of the given PfDE.

$$\mathbf{1.5} \quad (1 + yz)dx + x(z - x)dy - (1 + xy)dz = 0$$

We are given the Pfaffian differential equation:

$$(1 + yz) \, dx + x(z - x) \, dy - (1 + xy) \, dz = 0 \tag{1}$$

Lets define the vector $\vec{X} = (P, Q, R)$, where:

$$P = 1 + yz, \quad Q = x(z - x), \quad R = -(1 + xy)$$

Lets check integrability by computing $\vec{X} \cdot (\nabla \times \vec{X})$

$$\begin{aligned}\vec{X} \cdot (\nabla \times \vec{X}) &= \begin{vmatrix} P & Q & R \\ \frac{\partial}{\partial x} & \frac{\partial}{\partial y} & \frac{\partial}{\partial z} \\ P & Q & R \end{vmatrix} = \begin{vmatrix} 1+yz & x(z-x) & -(1+xy) \\ \frac{\partial}{\partial x} & \frac{\partial}{\partial y} & \frac{\partial}{\partial z} \\ 1+yz & x(z-x) & -(1+xy) \end{vmatrix} \\ &= (1+yz)(-x-x) - x(z-x)(-y-y) - (1+xy)(z-2x-z) \\ &= -2x(1+yz) + 2xy(z-x) + 2x(1+xy) \\ &= (-2x - 2xyz) + 2xyz - 2x^2y + 2x + 2x^2y \\ \vec{X} \cdot (\nabla \times \vec{X}) &= 0\end{aligned}$$

Since $\vec{X} \cdot (\nabla \times \vec{X}) = 0$, the Pfaffian differential equation is **integrable**.

Let $y = \text{constant}$, $\Rightarrow dy = 0$

Then the given PfDE reduces to:

$$\begin{aligned}(1+yz)dx - (1+xy)dz &= 0 \\ \Rightarrow \frac{dx}{1+xy} &= \frac{dz}{1+yz}\end{aligned}$$

Integrating while treating y as constant:

$$\begin{aligned}\int \frac{dx}{1+xy} &= \int \frac{dz}{1+yz} \\ \Rightarrow \frac{1}{y} \ln(1+xy) &= \frac{1}{y} \ln(1+yz) + C \\ \Rightarrow \frac{1+xy}{1+yz} &= \phi(y)\end{aligned}\tag{2}$$

Now set $z = \alpha = 1$, hence $dz = 0$

So the original PfDE becomes:

$$\begin{aligned}(1+y)dx + x(1-x)dy &= 0 \\ \Rightarrow \frac{dx}{x(1-x)} &= -\frac{dy}{1+y}\end{aligned}$$

Integrating on both sides, we get

$$\begin{aligned}\ln(x) - \ln(1-x) &= -\ln(1+y) + C_2 \\ \Rightarrow \ln\left(\frac{x(1+y)}{(1-x)}\right) &= C_2\end{aligned}$$

Exponentially both sides

$$\frac{x(1+y)}{1-x} = C, \quad \text{where } C = e^{C_2} \quad (3)$$

Substituting $z = 1$ in equation (2)

$$\frac{1+xy}{1+y} = \phi(y) \quad (4)$$

Also from equation (3)

$$\begin{aligned} x(1+y) &= C - Cx \\ \Rightarrow x &= \frac{C}{1+y+C} \end{aligned}$$

Using this value of x in equation (4), we get

$$\begin{aligned} \frac{1}{1+y} + \frac{Cy}{1+y+C} &= \phi(y) \\ \Phi(y) &= \frac{1+C}{1+y+C} \end{aligned}$$

Substituting $\phi(y)$ in equation (2) we get

$$\frac{1+xy}{1+yz} = \frac{1+C}{1+y+C}$$

This is the required general solution of given PfDE

$$\mathbf{1.6} \quad y(x+4)(y+z)dx - x(y+3z)dy + 2xydz = 0$$

We are given the Pfaffian differential equation:

$$y(x+4)(y+z)dx - x(y+3z)dy + 2xydz = 0 \quad (1)$$

Let us define the vector $\vec{X} = (P, Q, R)$, where:

$$P = y(x+4)(y+z), \quad Q = -x(y+3z), \quad R = 2xy$$

Let us check integrability by computing $\vec{X} \cdot (\nabla \times \vec{X})$:

$$\vec{X} \cdot (\nabla \times \vec{X}) = \begin{vmatrix} P & Q & R \\ \frac{\partial}{\partial x} & \frac{\partial}{\partial y} & \frac{\partial}{\partial z} \\ P & Q & R \end{vmatrix} = \begin{vmatrix} y(x+4)(y+z) & -x(y+3z) & 2xy \\ \frac{\partial}{\partial x} & \frac{\partial}{\partial y} & \frac{\partial}{\partial z} \\ y(x+4)(y+z) & -x(y+3z) & 2xy \end{vmatrix}$$

$$\begin{aligned}
&= y(x+4)(y+z)(2x+3x) - (-x(y+3z))(2y-y(x+4)) \\
&\quad + 2xy(-(y+3z)-(x+4)(2y+z)) \\
&= 5xy(x+4)(y+z) - xy(y+3z)(x+2) + 2xy(-9y-7z-2xy-xz) \\
&= xy[5xy+5xz+20y+20z-xy-2y-3xz-6z-18y-14z-4xy-2xz] \\
&\vec{X} \cdot (\nabla \times \vec{X}) = 0
\end{aligned}$$

Since $\vec{X} \cdot (\nabla \times \vec{X}) = 0$, the Pfaffian differential equation is **integrable**.
Let $x = \text{constants}$ this implies $dx = 0$
Then the given PfDE reduced to

$$\begin{aligned}
-x(y+3z)dy + 2xydz &= 0 \\
2xydz &= x(y+3z)dy \\
\frac{dz}{dy} &= \frac{y+3z}{2y} \\
\frac{dz}{dy} - \frac{3z}{2y} &= \frac{1}{2}
\end{aligned}$$

This is linear in z , and the integrating factor is

$$\mu(y) = \exp\left(-\int \frac{3}{2y} dy\right) = \exp\left(-\frac{3}{2} \ln y\right) = y^{-\frac{3}{2}}.$$

Multiplying the above ODE by μ :

$$\begin{aligned}
y^{-\frac{3}{2}} \frac{dz}{dy} - \frac{3}{2y} y^{-\frac{3}{2}} z &= \frac{1}{2} y^{-\frac{3}{2}} \\
\frac{d}{dy} (z y^{-\frac{3}{2}}) &= \frac{1}{2} y^{-\frac{3}{2}}
\end{aligned}$$

Integrating both sides:

$$\begin{aligned}
z y^{-\frac{3}{2}} &= \frac{1}{2} \int y^{-\frac{3}{2}} dy + C(x) \\
&= \frac{1}{2} \left(\frac{y^{-\frac{1}{2}}}{-\frac{1}{2}} \right) + \phi(x)
\end{aligned}$$

$$\frac{z+y}{y^{-\frac{3}{2}}} = \phi(x) \tag{2}$$

Now set $y = \alpha = 1$ this gives $dy = 0$
Then the given PfDE becomes

$$(x + 4)(1 + z) dx + 2x dz = 0$$

$$\frac{x + 4}{2x} dx = -\frac{dz}{1 + z}$$

$$\left(\frac{1}{2} + \frac{2}{x}\right) dx = -\frac{dz}{1 + z}$$

Integrating we get

$$\frac{1}{2} x + 2 \ln(x) = -\ln(1 + z) + C_1, \quad C_1 \text{ is an arbitrary constant}$$

Exponentiating both sides

$$x^2(1 + z) = C e^{-\frac{1}{2}}, \quad C = e^{C_1}$$

$$x^2(1 + z) = C \tag{3}$$

Substituting $y = 1$ in (2) we get

$$\phi(x) = 1 + z \tag{4}$$

From (3):

$$z = \frac{C}{x^2} e^{-\frac{x}{2}} - 1$$

Substituting this into (4) gives

$$\phi(x) = \frac{C}{x^2} e^{-\frac{x}{2}}$$

Hence equation (2) becomes

$$\frac{y + z}{y^{-\frac{3}{2}}} = \frac{C}{x^2} e^{-\frac{x}{2}},$$

$$x^2 \frac{y + z}{y^{-\frac{3}{2}} e^{-\frac{x}{2}}} = C.$$

This is the required first integrals of the given PfDE.

$$\mathbf{1.7} \quad yzdx + (x^2y - zx)dy + (x^2z - xy)dz = 0$$

We are given the Pfaffian differential equation:

$$yzdx + (x^2y - zx)dy + (x^2z - xy)dz = 0 \quad (1)$$

Let us define the vector $\vec{X} = (P, Q, R)$, where:

$$P = yz, \quad Q = x^2y - zx, \quad R = x^2z - xy$$

Let us check integrability by computing $\vec{X} \cdot (\nabla \times \vec{X})$:

$$\begin{aligned} \vec{X} \cdot (\nabla \times \vec{X}) &= \begin{vmatrix} P & Q & R \\ \frac{\partial}{\partial x} & \frac{\partial}{\partial y} & \frac{\partial}{\partial z} \\ P & Q & R \end{vmatrix} = \begin{vmatrix} yz & x^2y - xz & x^2z - xy \\ \frac{\partial}{\partial x} & \frac{\partial}{\partial y} & \frac{\partial}{\partial z} \\ yz & x^2y - xz & x^2z - xy \end{vmatrix} \\ &= yz((-x) - (-x)) - (x^2y - xz)((2xz - y) - y) + (x^2z - xy)((2xy - z) - z) \\ &= yz \cdot 0 - (x^2y - xz)2(xz - y) + (x^2z - xy)2(xy - z) \\ &= 2 \left[-(x^2y - xz)(xz - y) + (x^2z - xy)(xy - z) \right] \\ &= 0 \end{aligned}$$

Since $\vec{X} \cdot (\nabla \times \vec{X}) = 0$, so the given PfDE is integrable.

Set $y = \text{constant} \Rightarrow dy = 0$

Then the original equation simplifies to

$$\begin{aligned} yzdx + (x^2z - xy)dz &= 0 \\ \frac{z}{x}dx + \left(\frac{xz}{y} - 1 \right)dz &= 0 \\ \frac{z}{x}dx &= \left(1 - \frac{xz}{y} \right)dz \end{aligned}$$

So,

$$\frac{dx}{dz} = \frac{x}{z} - \frac{x^2}{y} \quad (\text{Bernoulli equation in } x)$$

Let $u = \frac{1}{x}$, so

$$\frac{du}{dz} = -\frac{1}{x^2} \frac{dx}{dz} \Rightarrow -\frac{1}{u^2} \frac{du}{dz} = \frac{1}{uz} - \frac{1}{y}$$

Multiplying both sides by $-u^2$:

$$\frac{du}{dz} + \frac{u}{z} = \frac{1}{y} \quad (\text{Linear ODE})$$

Integrating factor:

$$\mu = e^{\int \frac{1}{z} dz} = z$$

Multiply through by z :

$$z \frac{du}{dz} + u = \frac{z}{y} \Rightarrow \frac{d}{dz}(uz) = \frac{z}{y}$$

Integrate:

$$uz = \frac{1}{y} \int z dz = \frac{z^2}{2y} + \phi(y), \phi(y) \text{ is function of } y \text{ since } y \text{ is held constant}$$

Substitute $u = \frac{1}{x}$:

$$\phi(x) = \frac{z}{x} - \frac{z^2}{2y} \tag{2}$$

Again Set $z = 1 \Rightarrow dz = 0$

The equation becomes:

$$y dx + (x^2 y - x) dy = 0$$

$$dx + \left(x^2 - \frac{x}{y}\right) dy = 0$$

$$\frac{dx}{dy} = -x^2 + \frac{x}{y} \quad (\text{Bernoulli equation in } x)$$

Let $v = \frac{1}{x}$, so

$$\frac{dv}{dy} = -\frac{1}{x^2} \frac{dx}{dy} \Rightarrow -\frac{1}{v^2} \frac{dv}{dy} = -v^{-2} + \frac{1}{vy}$$

Multiply both sides by $-v^2$:

$$\frac{dv}{dy} + \frac{v}{y} = 1 \quad (\text{Linear ODE})$$

Integrating factor:

$$\mu = e^{\int \frac{1}{y} dy} = y$$

Multiply above ODE by y:

$$y \frac{dv}{dy} + v = y$$

$$\frac{d}{dy}(vy) = y$$

Integrate:

$$vy = \frac{y^2}{2} + C, \text{ where } C \text{ is an arbitrary constant}$$

Substituting $v = \frac{1}{x}$

$$\frac{y}{x} - \frac{y^2}{2} = C \quad (3)$$

Using $z = 1$ in equation (2) we get

$$\phi(x) = \frac{1}{x} - \frac{1}{2y} \quad (4)$$

From equation (3) $\frac{1}{x} = \frac{y}{2} + \frac{C}{y}$ and using this value in equation (4)

$$\phi(y) = \left(\frac{y}{2} + \frac{C}{y}\right) - \frac{1}{2y}$$

$$\phi(x) = \frac{y}{2} + \frac{2C-1}{2y}$$

Hence Equation (2) becomes

$$\frac{z}{x} - \frac{z^2}{2y} = \frac{y}{2} + \frac{2C-1}{2y}$$

$$\frac{2yz}{x} - z^2 = y^2 + 2C - 1$$

$$\frac{2yz}{x} = y^2 + z^2 + 2C - 1$$

$$2xyz = x(y^2 + z^2 + C_1), \text{ where } C_1 = 2C-1$$

$$x(y^2 + z^2) - 2yz = -C_1x$$

$$y^2 + z^2 - \frac{2yz}{x} = C_2, \text{ where } C_2 = -C_1$$

This is the require primitives of given PfDE

1.8 $2yzdx - 2xzdy - (x^2 - y^2)(z - 1)dz = 0$

We are given the Pfaffian differential equation:

$$2yz dx - 2xz dy - (x^2 - y^2)(z - 1) dz = 0 \quad (1)$$

Let us define the vector $\vec{X} = (P, Q, R)$, where:

$$P = 2yz, \quad Q = -2xz, \quad R = -(x^2 - y^2)(z - 1)$$

Let us check integrability by computing $\vec{X} \cdot (\nabla \times \vec{X})$:

$$\begin{aligned} \vec{X} \cdot (\nabla \times \vec{X}) &= \begin{vmatrix} P & Q & R \\ \frac{\partial}{\partial x} & \frac{\partial}{\partial y} & \frac{\partial}{\partial z} \\ P & Q & R \end{vmatrix} = \begin{vmatrix} 2yz & -2xz & -(x^2 - y^2)(z - 1) \\ \frac{\partial}{\partial x} & \frac{\partial}{\partial y} & \frac{\partial}{\partial z} \\ 2yz & -2xz & -(x^2 - y^2)(z - 1) \end{vmatrix} \\ &= 2yz \left(\frac{\partial}{\partial y} R - \frac{\partial}{\partial z} Q \right) - (-2xz) \left(\frac{\partial}{\partial x} R - \frac{\partial}{\partial z} P \right) + [-(x^2 - y^2)(z - 1)] \left(\frac{\partial}{\partial x} Q - \frac{\partial}{\partial y} P \right) \\ &= 2yz [2y(z - 1) - (-2x)] + 2xz [2x(z - 1) - 2z] - (x^2 - y^2)(z - 1) [-2z - 2z] \\ &= 2yz(2y(z - 1) + 2x) + 2xz(2x(z - 1) - 2z) + 4z(x^2 - y^2)(z - 1) \\ &= [4xyz + 4y^2z(z - 1)] + [-4xyz - 4x^2z(z - 1)] + [4z(x^2 - y^2)(z - 1)] \\ &= 4y^2z(z - 1) - 4x^2z(z - 1) + 4z(x^2 - y^2)(z - 1) \\ &= 0 \end{aligned}$$

Since $\vec{X} \cdot (\nabla \times \vec{X}) = 0$, the given PfDE is integrable.

Divide the original Pfaffian by $x^2 + y^2$:

$$\frac{2yz}{x^2 + y^2} dx - \frac{2xz}{x^2 + y^2} dy - \frac{(x^2 - y^2)(z - 1)}{x^2 + y^2} dz = 0.$$

Lets introduce the cylindrical coordinates $x = r \cos \theta$, $y = r \sin \theta$, $x^2 + y^2 = r^2$
Then

$$\begin{aligned} x^2 + y^2 &= r^2 \\ x^2 - y^2 &= r^2 \cos(2\theta) \\ dx &= \cos(\theta) dr - r \sin(\theta) d\theta \\ dy &= \sin(\theta) dr + r \cos(\theta) d\theta \end{aligned}$$

Substituting these values, we get

$$\begin{aligned}
& \frac{2z(r \sin(\theta)(\cos(\theta) dr - r \sin(\theta) d\theta) - r \cos(\theta)(\sin(\theta) dr + r \cos(\theta) d\theta))}{r^2} \\
& - \frac{r^2 \cos(2\theta)(z-1)}{r^2} dz = 0 \\
& \frac{2zr(\sin \theta \cos \theta dr - r \sin^2 \theta d\theta - \sin \theta \cos \theta dr - r \cos^2 \theta d\theta)}{r^2} - \cos(2\theta)(z-1) dz = 0 \\
& \frac{2zr(-r(\sin^2 \theta + \cos^2 \theta) d\theta)}{r^2} - \cos(2\theta)(z-1) dz = 0 \\
& - 2z d\theta - \cos(2\theta)(z-1) dz = 0 \\
& - 2z d\theta = \cos 2\theta(z-1) dz
\end{aligned}$$

Separating variables

$$\frac{d\theta}{\cos 2\theta} = -\frac{z-1}{2z} dz$$

Integrating both sides:

$$\begin{aligned}
\int \sec 2\theta d\theta &= -\frac{1}{2} \int \frac{z-1}{z} dz + C \quad \text{where } C \text{ is an arbitrary constant} \\
\frac{1}{2} \ln(\sec 2\theta + \tan 2\theta) &= -\frac{1}{2} \int \left(1 - \frac{1}{z}\right) dz + C \\
\ln(\sec 2\theta + \tan 2\theta) &= z - \ln(z) + C
\end{aligned}$$

Substituting back the Cartesian coordinates:

$$\sec 2\theta = \frac{1}{\cos 2\theta} = \frac{r^2}{x^2 + y^2} \quad \text{and} \quad \tan 2\theta = \frac{2 \sin \theta \cos \theta}{\cos^2 \theta - \sin^2 \theta}$$

$$\text{Hence, } \sec 2\theta + \tan 2\theta = \frac{r^2 + 2xy}{x^2 - y^2} = \frac{x^2 + 2xy + y^2}{x^2 - y^2} = \frac{(x+y)^2}{x^2 - y^2}$$

So the solution becomes

$$\ln \left(\frac{(x+y)^2}{x^2 - y^2} \right) = z - \ln(z) + C$$

Exponentiating both sides

$$\frac{(x+y)^2}{x^2 - y^2} = ze^{-z} e^C$$

$$\frac{x+y}{z(x-y)} = e^{-z} K \quad \text{where } K = e^C$$

This is the required primitive.